---
title: Ex. 5.4
linktitle: Ex 5.4
type: book
date: "2021-01-02T00:00:00+01:00"
# Prev/next pager order (if `docs_section_pager` enabled in `params.toml`)
weight: 1
toc: false
---

???+ question "Ex. 5.4"
    Consider the truncated power series representation for cubic splines with $K$ interior knots. Let 
	
    \begin{equation}
		f(X) = \sum_{j=0}^3\beta_jX^j + \sum_{k=1}^K\theta_k(X-\xi_k)_{+}^3.\non
	\end{equation}
	
    Prove that the natural boundary conditions for natural cubic splines (Section 5.2.1) imply the following linear constraints on the coefficients:
	
    \begin{eqnarray}
	    \beta_2 = 0, \ \  \sum_{k=1}^K\theta_k = 0\non\\
	    \beta_3 = 0, \ \  \sum_{k=1}^K\xi_k\theta_k=0.\non
	\end{eqnarray}
	
    Hence derive the basis (5.4) and (5.5).

??? done "Soln. 5.4"
    When $X<\xi_1$, $f(X) = \beta_0 + \beta_1X + \beta_2X^2 + \beta_3X^3$, since $f(X)$ is linear when $X < \xi_1$, we have $\beta_2=0$ and $\beta_3=0$.

	When $X > \xi_K$, we have
	
    \begin{eqnarray}
	    f(X) &=& \sum_{j=0}^3\beta_jX^j + \sum_{k=1}^K\theta_k(X-\xi_k)^3\non\\
	    &=&\beta_0 + \beta_1X + 3\left(\sum_{k=1}^K\theta_k\xi_k^2\right) X - 3\left(\sum_{k=1}^K\theta_k\xi_k\right)X^2 + \left(\sum_{k=1}^K\theta_k\right)X^3.\non
	\end{eqnarray}

	Since $f(X)$ is linear when $X > \xi_K$, we have
	
    \begin{equation}
	\label{eq:5-4a}
		\sum_{k=1}^K\theta_k = 0 \text{ and } \sum_{k=1}^K\theta_k\xi_k = 0. 
	\end{equation}

	To derive (5.4) and (5.5) in the text, we need to rewrite $f(X)$ as a series summation, in the form of $\sum_k\alpha_k N_k(X)$, defined in (5.4) and (5.5). It's easy to see that for $N_1(X)$ and $N_2(X)$, we have $\alpha_1 = \beta_1$ and $\alpha_2 = \beta_2$. By comparing the coefficient of $(X-\xi_k)_+^3$ for each $k \le K-2$, we see that $\alpha_k = (\xi_K-\xi_k)\theta_k$. It remains to verify that
	
    \begin{equation}
	 	\sum_{k=1}^{K-2}\alpha_kN_{k+2}(X) = \sum_{k=1}^K\theta_k(X-\xi_k)_{+}^3.\non
	 \end{equation} 

	We have
	
    \begin{eqnarray}
	    &&\sum_{k=1}^{K-2}\alpha_kN_{k+2}(X)\non\\
	    &=& \sum_{k=1}^{K-2}(\xi_K-\xi_k)\theta_k\left[\frac{(X-\xi_k)_+^3-(X-\xi_K)_+^3}{\xi_K-\xi_k} - \frac{(X-\xi_{K-1})_+^3-(X-\xi_K)_+^3}{\xi_K-\xi_{K-1}}\right]\non\\
	    &=&\sum_{k=1}^{K-2}\theta_k(x-\xi_k)_+^3 -\left(\sum_{k=1}^{K-2}\theta_k\right)(x-\xi_K)_+^3 \non\\
	    && - \frac{1}{\xi_K-\xi_{K-1}}\left[\xi_K\left(\sum_{k=1}^{K-2}\theta_k\right) - \sum_{k=1}^{K-2}\xi_k\theta_k\right][(X-\xi_{K-1})_+^3-(X-\xi_K)_+^3].\non
	\end{eqnarray}
	
    Note that by $\eqref{eq:5-4a}$, we have $\sum_{k=1}^{K-2}\theta_k=-\theta_{K-1}-\theta_K$ and $\sum_{k=1}^{K-2}\xi_k\theta_k=-\theta_{K-1}\xi_{K-1} - \theta_K\xi_K$, the summation above becomes

	\begin{eqnarray}
	    && \sum_{k=1}^{K-2}\theta_k(x-\xi_k)_+^3 + (\theta_{K-1}+\theta_K)(x-\xi_K)_+^3 \non\\
	    && - \frac{(-\xi_K\theta_{K-1}-\xi_K\theta_K + \xi_{K-1}\theta_{K-1} + \xi_K\theta_K)}{\xi_K-\xi_{K-1}}[(X-\xi_{K-1})_+^3-(X-\xi_K)_+^3]\non\\
		&=& \sum_{k=1}^{K-2}\theta_k(x-\xi_k)_+^3 + (\theta_{K-1}+\theta_K)(x-\xi_K)_+^3\non\\
		&& + \theta_{K-1}[(X-\xi_{K-1})_+^3-(X-\xi_K)_+^3]\non\\
	    &=& \sum_{k=1}^K\theta_k(x-\xi_k)_+^3.\non
	\end{eqnarray}
    
	Now the proof is complete. 